src/Contracts/Flex/Functions/FuncSig.v
@@ -1,0 +1,37 @@
+Require Import UMLang.SolidityNotations2.
+Require Import UMLang.SML_NG28.
+Require Import UrsusTVM.tvmNotations.
+
+Require Import Contracts.Flex.ClassTypes.
+Require Import Contracts.Flex.Ledger .
+
+Module Spec (xt: XTypesSig) (sm: StateMonadSig).
+
+Module Export ClassTypesForFuncSig := ClassTypes xt sm .
+Module LedgerModuleForFuncSig := Ledger xt sm .
+Module Export tvmNotationsModule := tvmNotations xt sm LedgerModuleForFuncSig.
+(*ничего не импортируем после этой строчки*)
+
+Module Type SpecSig.
+
+ Parameter Flex_Ф_constructor : XInteger256 -> XInteger128 -> XInteger128 -> XInteger128 -> XInteger128 -> XInteger128 -> XInteger128 -> XInteger8 -> XAddress -> UExpression PhantomType false . 
+ Parameter Flex_Ф_setPairCode : XCell -> UExpression PhantomType true . 
+ Parameter Flex_Ф_setXchgPairCode : XCell -> UExpression PhantomType true . 
+ Parameter Flex_Ф_setPriceCode : XCell -> UExpression PhantomType true . 
+ Parameter Flex_Ф_setXchgPriceCode : XCell -> UExpression PhantomType true . 
+ Parameter Flex_Ф_isFullyInitialized : UExpression XBool false . 
+ Parameter Flex_Ф_getTonsCfg : UExpression TonsConfigStateLRecord false . 
+ Parameter Flex_Ф_getTradingPairCode : UExpression XCell false . 
+ Parameter Flex_Ф_getXchgPairCode : UExpression XCell false . 
+ Parameter Flex_Ф_getSellPriceCode : XAddress -> UExpression XCell true . 
+ Parameter Flex_Ф_getXchgPriceCode : XAddress -> XAddress -> UExpression XCell true . 
+ Parameter Flex_Ф_getSellTradingPair : XAddress -> UExpression XAddress false . 
+ Parameter Flex_Ф_getXchgTradingPair : XAddress -> XAddress -> UExpression XAddress false . 
+ Parameter Flex_Ф_getDealsLimit : UExpression XInteger8 false . 
+ Parameter Flex_Ф_getNotifyAddr : UExpression XAddress false . 
+ Parameter Flex_Ф__fallback : XCell -> UExpression XInteger false . 
+
+End SpecSig.
+
+
+End Spec.  
