src/Contracts/Flex/Ledger.v
@@ -1,0 +1,285 @@
+ Require Import Coq.Program.Basics. 
+
+Require Import String. 
+Require Import FinProof.Types.IsoTypes. 
+Require Import FinProof.Common. 
+Require Import FinProof.MonadTransformers21. 
+
+Require Import FinProof.ProgrammingWith.  
+Require Import UMLang.UrsusLib. 
+Require Import UMLang.SolidityNotations2. 
+Require Import UMLang.ClassGenerator.ClassGenerator.
+Require Import UrsusTVM.tvmFunc. 
+
+Require Import Project.CommonTypes.
+
+Require Import Contracts.Flex.ClassTypes.
+Require Import Contracts.Flex.Interface.
+
+Local Open Scope record. 
+Local Open Scope program_scope.
+Local Open Scope xlist_scope.
+
+(* 1 *) Inductive MessagesAndEventsFields := | MessagesAndEvents_ι_field_1 | MessagesAndEvents_ι_field_2 | MessagesAndEvents_ι_field_3 | MessagesAndEvents_ι_field_4 .
+(* 1 *) Inductive ContractFields := | deployer_pubkey_ 
+                                    | tons_cfg_ 
+                                    | pair_code_ 
+                                    | xchg_pair_code_ 
+                                    | price_code_ 
+                                    | xchg_price_code_ 
+                                    | deals_limit_ 
+                                    | notify_addr_ .
+(* 1 *) Inductive LocalStateFieldsI := | _int | _intIndex | _optcell | _optcellIndex | _tpladdressaddress | _tpladdressaddressIndex | _uint256 | _uint256Index | _uint128 | _uint128Index | _uint8 | _uint8Index | _address | _addressIndex | _cell | _cellIndex | _XchgPair | _XchgPairIndex | _TradingPair | _TradingPairIndex |(*  _tplStateInituint256 | _tplStateInituint256Index | *) _bool | _boolIndex .
+(* 1 *) Inductive LedgerFieldsI := | _Contract | _ContractCopy | _VMState | _MessagesAndEvents | _MessagesAndEventsCopy | _LocalState | _LocalStateCopy .
+
+ Module Ledger (xt: XTypesSig) (sm: StateMonadSig) <: ClassSigTVM xt sm. 
+ Module Import SolidityNotationsForLedger := SolidityNotations xt sm.  
+ Module Export VMStateModule := VMStateModule xt sm. 
+ Module Export TypesModuleForLedger := ClassTypes xt sm .
+
+(* 2 *) Definition MessagesAndEventsStateL : list Type := 
+ [ ( XInteger ) : Type ; 
+ ( XBool ) : Type ; 
+ ( XCell ) : Type ; 
+ ( ( XHMap XInteger XInteger ) ) : Type ] .
+GeneratePruvendoRecord MessagesAndEventsStateL MessagesAndEventsFields . 
+  Opaque MessagesAndEventsStateLRecord . 
+
+(* 2 *) Definition ContractL : list Type := 
+ [ ( XInteger256 ) : Type ; 
+ ( TonsConfigStateLRecord ) : Type ; 
+ ( XMaybe XCell ) : Type ; 
+ ( XMaybe XCell ) : Type ; 
+ ( XMaybe XCell ) : Type ; 
+ ( XMaybe XCell ) : Type ; 
+ ( XInteger8 ) : Type ; 
+ ( XAddress ) : Type ] .
+GeneratePruvendoRecord ContractL ContractFields . 
+ Opaque ContractLRecord . 
+(* GeneratePruvendoRecord TradingPairStateL TradingPairFields . 
+ Opaque TradingPairStateLRecord . 
+GeneratePruvendoRecord XchgPairStateL XchgPairFields . 
+ Opaque XchgPairStateLRecord . *) 
+
+(* 2 *) Definition LocalStateL : list Type := 
+ [ ( XHMap (string*nat) XInteger ) : Type ; 
+ ( XHMap string nat ) : Type ; 
+ ( XHMap (string*nat) ( XMaybe XCell ) ) : Type ; 
+ ( XHMap string nat ) : Type ; 
+ ( XHMap (string*nat) ( XAddress * XAddress ) ) : Type ; 
+ ( XHMap string nat ) : Type ; 
+ ( XHMap (string*nat) XInteger256 ) : Type ; 
+ ( XHMap string nat ) : Type ; 
+ ( XHMap (string*nat) XInteger128 ) : Type ; 
+ ( XHMap string nat ) : Type ; 
+ ( XHMap (string*nat) XInteger8 ) : Type ; 
+ ( XHMap string nat ) : Type ; 
+ ( XHMap (string*nat) XAddress ) : Type ; 
+ ( XHMap string nat ) : Type ; 
+ ( XHMap (string*nat) XCell ) : Type ; 
+ ( XHMap string nat ) : Type ; 
+ ( XHMap (string*nat) XchgPairStateLRecord ) : Type ; 
+ ( XHMap string nat ) : Type ; 
+ ( XHMap (string*nat) TradingPairStateLRecord ) : Type ; 
+ ( XHMap string nat ) : Type ; 
+(*  ( XHMap (string*nat) ( StateInitStateLRecord * XInteger256 ) ) : Type ; 
+ ( XHMap string nat ) : Type ;  *)
+ ( XHMap (string*nat) XBool ) : Type ; 
+ ( XHMap string nat ) : Type ] .
+GeneratePruvendoRecord LocalStateL LocalStateFieldsI .
+ Opaque LocalStateLRecord . 
+
+Check VMStateLRecord.
+
+(* 2 *) Definition LedgerL : list Type := 
+ [ ( ContractLRecord ) : Type ; 
+ ( ContractLRecord ) : Type ; 
+ ( VMStateLRecord ) : Type ; 
+ ( MessagesAndEventsStateLRecord ) : Type ; 
+ ( MessagesAndEventsStateLRecord ) : Type ; 
+ ( LocalStateLRecord ) : Type ; 
+ ( LocalStateLRecord ) : Type ] .
+GeneratePruvendoRecord LedgerL LedgerFieldsI .
+(***************************************)
+Transparent MessagesAndEventsStateLRecord .
+Transparent ContractLRecord .
+Transparent LocalStateLRecord .
+Transparent LedgerLRecord .
+
+Definition LedgerPruvendoRecord := LedgerLPruvendoRecord .
+Definition LedgerLocalState := LocalStateLRecord .
+Definition LedgerLocalFields := LocalStateFieldsI.
+Definition LedgerLocalPruvendoRecord := LocalStateLPruvendoRecord .
+Definition LocalEmbedded := LedgerLEmbeddedType _LocalState .
+Definition LocalCopyEmbedded := LedgerLEmbeddedType _LocalStateCopy.
+Definition LocalDefault : XDefault LocalStateLRecord := prod_default.
+Definition Ledger_LocalState := _LocalState.
+Definition Ledger_LocalStateCopy := _LocalStateCopy.
+Definition iso_local := _LocalStateIso.
+Definition Ledger := LedgerLRecord.
+Definition LedgerFields := LedgerFieldsI.
+
+(* Definition MessagesAndEvents := _MessagesAndEvents. *)
+
+
+Lemma LedgerFieldsDec: forall (m1 m2: LedgerFieldsI), {m1=m2}+{m1<>m2}.
+Proof.
+  intros.
+  decide equality.
+Defined.
+
+Lemma LocalCopySameType: field_type  Ledger_LocalState = 
+field_type Ledger_LocalStateCopy.
+Proof.
+  reflexivity.
+Defined.
+
+
+Class LocalStateField (X:Type): Type := 
+{
+    local_index_embedded:> EmbeddedType LocalStateLRecord (XHMap string nat) ;
+    local_state_field: LedgerLocalFields;
+    local_field_type_correct: field_type local_state_field = XHMap (string*nat)%type X;
+}.
+
+Definition LedgerVMStateEmbedded := LedgerLEmbeddedType _VMState . 
+Definition LedgerVMStateField := _VMState .
+Definition isoVMState := _VMStateIso.
+
+Definition LedgerMessagesEmbedded := LedgerLEmbeddedType _MessagesAndEvents . 
+Definition LedgerMessagesField := _MessagesAndEvents .
+Definition isoMessages := _MessagesAndEventsIso.
+Definition MessagesAndEvents := MessagesAndEventsStateLRecord .
+
+GenerateLocalStateInstances LocalStateL LocalStateFieldsI Build_LocalStateField LocalStateLEmbeddedType.
+#[global]
+ Declare Instance foo : LocalStateField (StateInitStateLRecord * XInteger256).
+
+Definition LocalStateField_XInteger := _intLocalField .
+Definition LocalStateField_XBool := _boolLocalField .
+Definition LocalStateField_XCell := _cellLocalField .
+
+(* Definition LedgerVMStateEmbedded := LedgerStateLEmbeddedType _VMState . 
+Definition LedgerVMStateField := _VMState .
+Definition isoVMState := _VMStateIso.
+
+GenerateLocalStateInstances LocalStateStateL LocalStateFieldsI Build_LocalStateField LocalStateStateLEmbeddedType.
+
+Definition LocalStateField_XInteger := _intLocalField .
+Definition LocalStateField_XBool := _boolLocalField .
+Definition LocalStateField_XCell := _cellLocalField .
+ *)
+
+
+
+(***************************************)
+(* Lemma MessagesAndEventsFields_noeq : forall (f1 f2:  MessagesAndEventsFields ) 
+         (v2: field_type f2) (r :  MessagesAndEventsStateLRecord  ) ,  
+f1 <> f2 -> 
+f1 {$$ r with f2 := v2 $$} = f1 r.
+Proof.
+  intros.
+  destruct f1; destruct f2; 
+  (revert r;     
+               apply (countable_prop_proof (T:= MessagesAndEventsStateLRecord ));
+               cbv;
+               first [reflexivity| contradiction]).
+Qed .
+Lemma TickTockFields_noeq : forall (f1 f2:  TickTockFields ) 
+         (v2: field_type f2) (r :  TickTockStateLRecord  ) ,  
+f1 <> f2 -> 
+f1 {$$ r with f2 := v2 $$} = f1 r.
+Proof.
+  intros.
+  destruct f1; destruct f2; 
+  (revert r;     
+               apply (countable_prop_proof (T:= TickTockStateLRecord ));
+               cbv;
+               first [reflexivity| contradiction]).
+Qed .
+Lemma StateInitFields_noeq : forall (f1 f2:  StateInitFields ) 
+         (v2: field_type f2) (r :  StateInitStateLRecord  ) ,  
+f1 <> f2 -> 
+f1 {$$ r with f2 := v2 $$} = f1 r.
+Proof.
+  intros.
+  destruct f1; destruct f2; 
+  (revert r;     
+               apply (countable_prop_proof (T:= StateInitStateLRecord ));
+               cbv;
+               first [reflexivity| contradiction]).
+Qed .
+Lemma TonsConfigFields_noeq : forall (f1 f2:  TonsConfigFields ) 
+         (v2: field_type f2) (r :  TonsConfigStateLRecord  ) ,  
+f1 <> f2 -> 
+f1 {$$ r with f2 := v2 $$} = f1 r.
+Proof.
+  intros.
+  destruct f1; destruct f2; 
+  (revert r;     
+               apply (countable_prop_proof (T:= TonsConfigStateLRecord ));
+               cbv;
+               first [reflexivity| contradiction]).
+Qed .
+Lemma FlexFields_noeq : forall (f1 f2:  FlexFields ) 
+         (v2: field_type f2) (r :  FlexStateLRecord  ) ,  
+f1 <> f2 -> 
+f1 {$$ r with f2 := v2 $$} = f1 r.
+Proof.
+  intros.
+  destruct f1; destruct f2; 
+  (revert r;     
+               apply (countable_prop_proof (T:= FlexStateLRecord ));
+               cbv;
+               first [reflexivity| contradiction]).
+Qed .
+Lemma TradingPairFields_noeq : forall (f1 f2:  TradingPairFields ) 
+         (v2: field_type f2) (r :  TradingPairStateLRecord  ) ,  
+f1 <> f2 -> 
+f1 {$$ r with f2 := v2 $$} = f1 r.
+Proof.
+  intros.
+  destruct f1; destruct f2; 
+  (revert r;     
+               apply (countable_prop_proof (T:= TradingPairStateLRecord ));
+               cbv;
+               first [reflexivity| contradiction]).
+Qed .
+Lemma XchgPairFields_noeq : forall (f1 f2:  XchgPairFields ) 
+         (v2: field_type f2) (r :  XchgPairStateLRecord  ) ,  
+f1 <> f2 -> 
+f1 {$$ r with f2 := v2 $$} = f1 r.
+Proof.
+  intros.
+  destruct f1; destruct f2; 
+  (revert r;     
+               apply (countable_prop_proof (T:= XchgPairStateLRecord ));
+               cbv;
+               first [reflexivity| contradiction]).
+Qed . *)
+(* Lemma LocalStateFields_noeq : forall (f1 f2:  LocalStateFieldsI ) 
+         (v2: field_type f2) (r :  LocalStateStateLRecord  ) ,  
+f1 <> f2 -> 
+f1 {$$ r with f2 := v2 $$} = f1 r.
+Proof.
+  intros.
+  destruct f1; destruct f2; 
+  (revert r;     
+               apply (countable_prop_proof (T:= LocalStateStateLRecord ));
+               cbv;
+               first [reflexivity| contradiction]).
+Qed . *)
+(* Lemma LedgerFields_noeq : forall (f1 f2:  LedgerFields ) 
+         (v2: field_type f2) (r :  LedgerStateLRecord  ) ,  
+f1 <> f2 -> 
+f1 {$$ r with f2 := v2 $$} = f1 r.
+Proof.
+  intros.
+  destruct f1; destruct f2; 
+  (revert r;     
+               apply (countable_prop_proof (T:= LedgerStateLRecord ));
+               cbv;
+               first [reflexivity| contradiction]).
+Qed . *)
+
+End Ledger .
