src/Contracts/FlexClient/Functions/Funcs.v
@@ -39,39 +39,13 @@ main _ :- coq.error "usage: AddLocalState <name> <term> <LocalStateField>".
 Elpi Typecheck.
 Elpi Export AddLocalState.
 
-Elpi Command TestDefinitions. 
-Elpi Accumulate lp:{{
-
-pred get_name i:string , o:term.
-get_name NameS NameG :-
-    coq.locate NameS GR ,
-    NameG = global GR . 
-
-pred constructors_names i:string , o:list constructor.
-constructors_names IndName Names :-
-  std.assert! (coq.locate IndName (indt GR)) "not an inductive type",
-  coq.env.indt GR _ _ _ _ Names _.
-
-pred coqlist->list i:term, o: list term.
-coqlist->list {{ [ ]%xlist }} [ ].
-coqlist->list {{ (lp:X::lp:XS)%xlist }} [X | M] :- coqlist->list XS M.
-coqlist->list X _ :- coq.say "error",
-                    coq.say X.
-
-main [ A ] :-
-  coq.say  A. 
-}}. 
-
-Elpi Typecheck.
  
-(* Module trainContractSpecModuleForFuncs := trainContractSpec XTypesModule StateMonadModule. *)
+Module Funcs (dc : ConstsTypesSig XTypesModule StateMonadModule) .
+ 
+Module Export FuncNotationsModuleForFuncs := FuncNotations XTypesModule StateMonadModule dc. 
+Export SpecModuleForFuncNotations.tvmNotationsModule.
 
-Module FlexClientFuncs (dc : ConstsTypesSig XTypesModule StateMonadModule) .
-
-Module Export FlexClientFuncNotationsModule := FlexClientFuncNotations XTypesModule StateMonadModule dc. 
-Import (* trainContractSpecModule(* ForFuncs *) *)tvmNotationsModule.
-
-Module FlexClientFuncsInternal (* <: trainContractSpecModule(* ForFuncs *).trainContractSpecSig *).
+Module FuncsInternal <: SpecModuleForFuncNotations.SpecSig. 
  
 Import UrsusNotations.
 Local Open Scope ursus_scope.
@@ -535,8 +509,8 @@ Defined .
 }}. *)
 
 
-End FlexClientFuncsInternal.
-End FlexClientFuncs.
+End FuncsInternal.
+End Funcs.
 
 
 
