src/Contracts/_Price/ClassTypes.v
@@ -1,0 +1,177 @@
+
+Require Import UMLang.SolidityNotations2.
+Require Import UMLang.UrsusLib.
+
+Require Import UrsusStdLib.stdFunc.
+Require Import UrsusStdLib.stdNotations.
+Require Import UrsusStdLib.stdFuncNotations.
+
+Require Import UrsusTVM.tvmFunc.
+Require Import UrsusTVM.tvmNotations.
+Require Import FinProof.ProgrammingWith.  
+Require Import UMLang.ClassGenerator.ClassGenerator.
+
+Require Import Project.CommonTypes.
+
+
+Module ClassTypes (xt: XTypesSig) (sm: StateMonadSig) .
+Module Import CommonTypes := Types xt sm.
+
+Local Open Scope xlist_scope.
+
+(* 1 *) Inductive TickTockFields := | TickTock_ι_tick | TickTock_ι_tock | TickTok_ι_1 .
+(* 1 *) Inductive StateInitFields := | StateInit_ι_split_depth | StateInit_ι_special | StateInit_ι_code | StateInit_ι_data | StateInit_ι_library .
+(* 1 *) Inductive addr_std_fixedFields := | addr_std_fixed_ι_workchain_id | addr_std_fixed_ι_address | addr_std_fixed_ι_1 .
+(* 1 *) Inductive TonsConfigFields := | TonsConfig_ι_transfer_tip3 | TonsConfig_ι_return_ownership | TonsConfig_ι_trading_pair_deploy | TonsConfig_ι_order_answer | TonsConfig_ι_process_queue | TonsConfig_ι_send_notify .
+(* 1 *) Inductive OrderRetFields := | OrderRet_ι_err_code | OrderRet_ι_processed | OrderRet_ι_enqueued .
+(* 1 *) Inductive SellArgsFields := | SellArgs_ι_amount | SellArgs_ι_receive_wallet | SellArgs_ι_1 .
+(* 1 *) Inductive OrderInfoFields := | OrderInfo_ι_original_amount | OrderInfo_ι_amount | OrderInfo_ι_account | OrderInfo_ι_tip3_wallet | OrderInfo_ι_client_addr | OrderInfo_ι_order_finish_time .
+(* 1 *) Inductive DetailsInfoFields := | DetailsInfo_ι_price | DetailsInfo_ι_min_amount | DetailsInfo_ι_sell_amount | DetailsInfo_ι_buy_amount .
+(* 1 *) Inductive Tip3ConfigFields := | Tip3Config_ι_name | Tip3Config_ι_symbol | Tip3Config_ι_decimals | Tip3Config_ι_root_public_key | Tip3Config_ι_root_address .
+(* 1 *) Inductive dealerFields := | dealer_ι_tip3root_ | dealer_ι_notify_addr_ | dealer_ι_price_ | dealer_ι_deals_limit_ | dealer_ι_tons_cfg_ | dealer_ι_sells_amount_ | dealer_ι_buys_amount_ | dealer_ι_ret_ .
+(* 1 *) Inductive process_retFields := | process_ret_ι_sells_amount | process_ret_ι_buys_amount | process_ret_ι_ret_ .
+(* 1 *) Inductive lend_ownership_infoFields := | lend_ownership_info_ι_owner | lend_ownership_info_ι_lend_balance | lend_ownership_info_ι_lend_finish_time .
+(* 1 *) Inductive allowance_infoFields := | allowance_info_ι_spender | allowance_info_ι_remainingTokens | allowance_info_ι_1 .
+(* 1 *) Inductive TONTokenWalletFields := | TONTokenWallet_ι_name_ | TONTokenWallet_ι_symbol_ | TONTokenWallet_ι_decimals_ | TONTokenWallet_ι_balance_ | TONTokenWallet_ι_root_public_key_ | TONTokenWallet_ι_wallet_public_key_ | TONTokenWallet_ι_root_address_ | TONTokenWallet_ι_owner_address_ | TONTokenWallet_ι_lend_ownership_ | TONTokenWallet_ι_code_ | TONTokenWallet_ι_allowance_ | TONTokenWallet_ι_workchain_id_ .
+(* 1 *) Inductive OrderInfoXchgFields := | OrderInfoXchg_ι_original_amount | OrderInfoXchg_ι_amount | OrderInfoXchg_ι_account | OrderInfoXchg_ι_tip3_wallet_provide | OrderInfoXchg_ι_tip3_wallet_receive | OrderInfoXchg_ι_client_addr | OrderInfoXchg_ι_order_finish_time .
+
+
+(* 2 *) Definition TickTockStateL : list Type := 
+ [ ( XBool ) : Type ; 
+ ( XBool ) : Type ;
+(XBool):Type ] .
+Elpi GeneratePruvendoRecord TickTockStateL TickTockFields . 
+ Opaque TickTockStateLRecord . 
+
+(* 2 *) Definition StateInitStateL : list Type := 
+ [ ( XMaybe XInteger ) : Type ; 
+ ( XMaybe TickTockStateLRecord ) : Type ; 
+ ( XMaybe XCell ) : Type ; 
+ ( XMaybe XCell ) : Type ; 
+ ( XMaybe XCell ) : Type ] .
+Elpi GeneratePruvendoRecord StateInitStateL StateInitFields . 
+ Opaque StateInitStateLRecord . 
+
+(* 2 *) Definition addr_std_fixedStateL : list Type := 
+ [ ( XInteger8 ) : Type ; 
+ ( XInteger256 ) : Type ;
+(XBool):Type ] . 
+Elpi GeneratePruvendoRecord addr_std_fixedStateL addr_std_fixedFields . 
+ Opaque addr_std_fixedStateLRecord . 
+
+(* 2 *) Definition TonsConfigStateL : list Type := 
+ [ ( XInteger128 ) : Type ; 
+ ( XInteger128 ) : Type ; 
+ ( XInteger128 ) : Type ; 
+ ( XInteger128 ) : Type ; 
+ ( XInteger128 ) : Type ; 
+ ( XInteger128 ) : Type ] .
+Elpi GeneratePruvendoRecord TonsConfigStateL TonsConfigFields . 
+ Opaque TonsConfigStateLRecord . 
+
+(* 2 *) Definition OrderRetStateL : list Type := 
+ [ ( XInteger32 ) : Type ; 
+ ( XInteger128 ) : Type ; 
+ ( XInteger128 ) : Type ] .
+Elpi GeneratePruvendoRecord OrderRetStateL OrderRetFields . 
+ Opaque OrderRetStateLRecord . 
+
+(* 2 *) Definition SellArgsStateL : list Type := 
+ [ ( XInteger128 ) : Type ; 
+ ( XAddress ) : Type ;
+(XBool):Type] .
+Elpi GeneratePruvendoRecord SellArgsStateL SellArgsFields . 
+ Opaque SellArgsStateLRecord . 
+
+(* 2 *) Definition OrderInfoStateL : list Type := 
+ [ ( XInteger128 ) : Type ; 
+ ( XInteger128 ) : Type ; 
+ ( XInteger128 ) : Type ; 
+ ( addr_std_fixedStateLRecord ) : Type ; 
+ ( addr_std_fixedStateLRecord ) : Type ; 
+ ( XInteger32 ) : Type ] .
+Elpi GeneratePruvendoRecord OrderInfoStateL OrderInfoFields . 
+ Opaque OrderInfoStateLRecord . 
+
+(* 2 *) Definition DetailsInfoStateL : list Type := 
+ [ ( XInteger128 ) : Type ; 
+ ( XInteger128 ) : Type ; 
+ ( XInteger128 ) : Type ; 
+ ( XInteger128 ) : Type ] .
+Elpi GeneratePruvendoRecord DetailsInfoStateL DetailsInfoFields . 
+ Opaque DetailsInfoStateLRecord . 
+
+(* 2 *) Definition Tip3ConfigStateL : list Type := 
+ [ ( XString ) : Type ; 
+ ( XString ) : Type ; 
+ ( XInteger8 ) : Type ; 
+ ( XInteger256 ) : Type ; 
+ ( XAddress ) : Type ] .
+Elpi GeneratePruvendoRecord Tip3ConfigStateL Tip3ConfigFields . 
+ Opaque Tip3ConfigStateLRecord . 
+
+(* 2 *) Definition dealerStateL : list Type := 
+ [ ( XAddress ) : Type ; 
+ ( XAddress ) : Type ; 
+ ( XInteger128 ) : Type ; 
+ ( XInteger ) : Type ; 
+ ( TonsConfigStateLRecord ) : Type ; 
+ ( XInteger128 ) : Type ; 
+ ( XInteger128 ) : Type ; 
+ ( XMaybe OrderRetStateLRecord ) : Type ] .
+Elpi GeneratePruvendoRecord dealerStateL dealerFields . 
+ Opaque dealerStateLRecord . 
+
+(* 2 *) Definition process_retStateL : list Type := 
+ [ ( XInteger128 ) : Type ; 
+ ( XInteger128 ) : Type ; 
+ ( XMaybe OrderRetStateLRecord ) : Type ] .
+Elpi GeneratePruvendoRecord process_retStateL process_retFields . 
+ Opaque process_retStateLRecord . 
+
+(* 2 *) Definition lend_ownership_infoStateL : list Type := 
+ [ ( XAddress ) : Type ; 
+ ( TokensType ) : Type ; 
+ ( XInteger32 ) : Type ] .
+Elpi GeneratePruvendoRecord lend_ownership_infoStateL lend_ownership_infoFields . 
+ Opaque lend_ownership_infoStateLRecord . 
+
+(* 2 *) Definition allowance_infoStateL : list Type := 
+ [ ( XAddress ) : Type ; 
+ ( TokensType ) : Type ;
+(XBool):Type] .
+Elpi GeneratePruvendoRecord allowance_infoStateL allowance_infoFields . 
+ Opaque allowance_infoStateLRecord . 
+
+(* 2 *) Definition TONTokenWalletStateL : list Type := 
+ [ ( XList XInteger8 ) : Type ; 
+ ( XList XInteger8 ) : Type ; 
+ ( XInteger8 ) : Type ; 
+ ( TokensType ) : Type ; 
+ ( XInteger256 ) : Type ; 
+ ( XInteger256 ) : Type ; 
+ ( XAddress ) : Type ; 
+ ( XMaybe XAddress ) : Type ; 
+ ( XMaybe lend_ownership_infoStateLRecord ) : Type ; 
+ ( XCell ) : Type ; 
+ ( XMaybe allowance_infoStateLRecord ) : Type ; 
+ ( XInteger8 ) : Type ] .
+Elpi GeneratePruvendoRecord TONTokenWalletStateL TONTokenWalletFields . 
+ Opaque TONTokenWalletStateLRecord . 
+
+(* 2 *) Definition OrderInfoXchgStateL : list Type := 
+ [ ( XInteger128 ) : Type ; 
+ ( XInteger128 ) : Type ; 
+ ( XInteger128 ) : Type ; 
+ ( addr_std_fixedStateLRecord ) : Type ; 
+ ( addr_std_fixedStateLRecord ) : Type ; 
+ ( addr_std_fixedStateLRecord ) : Type ; 
+ ( XInteger32 ) : Type ] .
+Elpi GeneratePruvendoRecord OrderInfoXchgStateL OrderInfoXchgFields . 
+ Opaque OrderInfoXchgStateLRecord . 
+
+
+
+
+End ClassTypes .
+ 
