src/Contracts/_Price/Ledger.v
@@ -1,0 +1,269 @@
+ Require Import Coq.Program.Basics. 
+
+Require Import String. 
+Require Import FinProof.Types.IsoTypes. 
+Require Import FinProof.Common. 
+Require Import FinProof.MonadTransformers21. 
+
+Require Import FinProof.ProgrammingWith.  
+Require Import UMLang.UrsusLib. 
+Require Import UMLang.SolidityNotations2. 
+Require Import UMLang.ClassGenerator.ClassGenerator.
+Require Import UrsusTVM.tvmFunc. 
+
+Require Import Project.CommonTypes.
+
+Require Import Contracts.Price.ClassTypes.
+Require Import Contracts.Price.Interface.
+
+Local Open Scope record. 
+Local Open Scope program_scope.
+Local Open Scope xlist_scope.
+
+
+(* 1 *) Inductive MessagesAndEventsFields := | MessagesAndEvents_ι_field_1 | MessagesAndEvents_ι_field_2 | MessagesAndEvents_ι_field_3 | MessagesAndEvents_ι_field_4 .
+(* 1 *) Inductive PriceFields := | Price_ι_price_ | Price_ι_sells_amount_ | Price_ι_buys_amount_ | Price_ι_flex_ | Price_ι_min_amount_ | Price_ι_deals_limit_ | Price_ι_notify_addr_ | Price_ι_workchain_id_ | Price_ι_tons_cfg_ | Price_ι_tip3_code_ | Price_ι_tip3cfg_ .
+(* 1 *) Inductive LocalStateFieldsI := 
+| LocalState_ι_cell 
+| LocalState_ι_cellIndex 
+| LocalState_ι_bool 
+| LocalState_ι_boolIndex 
+| LocalState_ι_int 
+| LocalState_ι_intIndex 
+ .
+(* 1 *) Inductive LedgerFieldsI := | Ledger_ι_Contract | Ledger_ι_ContractCopy | Ledger_ι_VMState | Ledger_ι_MessagesAndEvents | Ledger_ι_MessagesAndEventsCopy | Ledger_ι_LocalState | Ledger_ι_LocalStateCopy .
+
+ Module PriceClass (xt: XTypesSig) (sm: StateMonadSig) <: ClassSigTVM xt sm. 
+ Module Export SolidityNotationsClass := SolidityNotations xt sm. 
+ Module Export VMStateModule := VMStateModule xt sm. 
+ Module Export ClassTypesModule := ClassTypes xt sm .
+Import xt.
+Opaque Tip3ConfigStateLRecord .
+(* 2 *) Definition MessagesAndEventsStateL : list Type := 
+ [ ( XInteger ) : Type ; 
+ ( XBool ) : Type ; 
+ ( XCell ) : Type ; 
+ ( ( XHMap XInteger XInteger ) ) : Type ] .
+GeneratePruvendoRecord MessagesAndEventsStateL MessagesAndEventsFields . 
+  Opaque MessagesAndEventsStateLRecord . 
+
+(* 2 *) Definition PriceStateL : list Type := 
+ [ ( XInteger128 ) : Type ; 
+ ( XInteger128 ) : Type ; 
+ ( XInteger128 ) : Type ; 
+ ( addr_std_fixedStateLRecord ) : Type ; 
+ ( XInteger128 ) : Type ; 
+ ( XInteger8 ) : Type ; 
+ ( XAddress ) : Type ; 
+ ( XInteger8 ) : Type ; 
+ ( TonsConfigStateLRecord ) : Type ; 
+ ( XCell ) : Type ; 
+ ( Tip3ConfigStateLRecord ) : Type ] .
+GeneratePruvendoRecord PriceStateL PriceFields . 
+ Opaque PriceStateLRecord .
+
+(* 2 *) Definition LocalStateStateL : list Type := 
+ [  ( XHMap (string*nat) XCell) : Type ; 
+    ( XHMap string nat ) : Type ;
+    ( XHMap (string*nat) XBool) : Type ; 
+    ( XHMap string nat ) : Type ;
+    ( XHMap (string*nat) XInteger) : Type ;
+    ( XHMap string nat ) : Type  ] .
+
+GeneratePruvendoRecord LocalStateStateL LocalStateFieldsI . 
+ Opaque LocalStateStateLRecord .
+
+(* 2 *) Definition LedgerStateL : list Type := 
+ [ ( PriceStateLRecord ) : Type ; 
+ ( PriceStateLRecord ) : Type ; 
+ ( VMStateLRecord ) : Type ; 
+ ( MessagesAndEventsStateLRecord ) : Type ; 
+ ( MessagesAndEventsStateLRecord ) : Type ; 
+ ( LocalStateStateLRecord ) : Type ; 
+ ( LocalStateStateLRecord ) : Type ] .
+Elpi GeneratePruvendoRecord LedgerStateL LedgerFieldsI .
+
+Transparent TickTockStateLRecord .
+Transparent StateInitStateLRecord .
+Transparent addr_std_fixedStateLRecord .
+Transparent TonsConfigStateLRecord .
+Transparent OrderRetStateLRecord .
+Transparent SellArgsStateLRecord .
+Transparent OrderInfoStateLRecord .
+Transparent DetailsInfoStateLRecord .
+Transparent Tip3ConfigStateLRecord .
+Transparent PriceStateLRecord .
+Transparent dealerStateLRecord .
+Transparent process_retStateLRecord .
+Transparent lend_ownership_infoStateLRecord .
+Transparent allowance_infoStateLRecord .
+Transparent TONTokenWalletStateLRecord .
+Transparent OrderInfoXchgStateLRecord .
+
+Transparent VMStateLRecord.
+Transparent MessagesAndEventsStateLRecord.
+Transparent LocalStateStateLRecord.
+
+(***************************************)
+
+Definition LedgerPruvendoRecord := LedgerStateLPruvendoRecord .
+Definition LedgerLocalState := LocalStateStateLRecord .
+Definition LedgerLocalFields := LocalStateFieldsI.
+Definition LedgerLocalPruvendoRecord := LocalStateStateLPruvendoRecord .
+Definition LocalEmbedded := LedgerStateLEmbeddedType Ledger_ι_LocalState .
+Definition LocalCopyEmbedded := LedgerStateLEmbeddedType Ledger_ι_LocalStateCopy.
+Definition LocalDefault : XDefault LocalStateStateLRecord := prod_default.
+Definition Ledger_LocalState := Ledger_ι_LocalState.
+Definition Ledger_LocalStateCopy := Ledger_ι_LocalStateCopy.
+Definition iso_local := Ledger_ι_LocalStateIso.
+Definition Ledger := LedgerStateLRecord.
+Definition LedgerFields := LedgerFieldsI.
+
+Lemma LedgerFieldsDec: forall (m1 m2: LedgerFieldsI), {m1=m2}+{m1<>m2}.
+Proof.
+  intros.
+  decide equality.
+Defined.
+
+Lemma LocalCopySameType: field_type  Ledger_LocalState = 
+field_type Ledger_LocalStateCopy.
+Proof.
+  reflexivity.
+Defined.
+
+Class LocalStateField (X:Type): Type := 
+{
+    local_index_embedded:> EmbeddedType LocalStateStateLRecord (XHMap string nat) ;
+    local_state_field: LedgerLocalFields;
+    local_field_type_correct: field_type local_state_field = XHMap (string*nat)%type X;
+}.
+
+Declare Instance LocalState_ι_cell : LocalStateField XCell  .  
+ 
+ Declare Instance LocalState_ι_StateInit     : LocalStateField StateInitStateLRecord  .  
+ 
+ Declare Instance LocalState_ι_tplStateInituint256 : LocalStateField ( StateInitStateLRecord * XInteger256 )  .  
+ 
+ Declare Instance LocalState_ι_bool     : LocalStateField XBool  .  
+ 
+ Declare Instance LocalState_ι_uint32     : LocalStateField XInteger32  .  
+ 
+ Declare Instance LocalState_ι_Price     : LocalStateField PriceStateLRecord  .  
+ 
+ Declare Instance LocalState_ι_optuint128     : LocalStateField ( XMaybe XInteger128 )  .  
+ 
+ Declare Instance LocalState_ι_uint128     : LocalStateField XInteger128  .  
+ 
+ Declare Instance LocalState_ι_OrderInfo     : LocalStateField OrderInfoStateLRecord  .  
+ 
+ Declare Instance LocalState_ι_int     : LocalStateField XInteger  .  
+ 
+ Declare Instance LocalState_ι_optpair_unsigned_OrderInfo__     : LocalStateField ( XMaybe (XInteger * OrderInfoStateLRecord) )  .  
+ 
+ Declare Instance LocalState_ι_OrderRet     : LocalStateField OrderRetStateLRecord  .  
+ 
+ Declare Instance LocalState_ι_unsigned     : LocalStateField XInteger  .  
+ 
+ Declare Instance LocalState_ι_dealer     : LocalStateField dealerStateLRecord  .  
+ 
+ Declare Instance LocalState_ι_uint8     : LocalStateField XInteger8  .  
+ 
+ Declare Instance LocalState_ι_TonsConfig     : LocalStateField TonsConfigStateLRecord  .  
+ 
+ Declare Instance LocalState_ι_tplqueue_OrderInfouint128     : LocalStateField ( (XHMap XInteger OrderInfoStateLRecord) * XInteger128 )  .  
+ 
+ Declare Instance LocalState_ι_addr_std_fixed     : LocalStateField addr_std_fixedStateLRecord  .  
+ 
+ Declare Instance LocalState_ι_Grams     : LocalStateField XInteger256 (* Grams *)  .  
+ 
+ Declare Instance LocalState_ι_SellArgs     : LocalStateField SellArgsStateLRecord  .  
+ 
+ Declare Instance LocalState_ι_address     : LocalStateField XAddress  .  
+ 
+ Declare Instance LocalState_ι_DetailsInfo     : LocalStateField DetailsInfoStateLRecord  .  
+ 
+ Declare Instance LocalState_ι_dict_arrayOrderInfo     : LocalStateField ( XHMap XInteger OrderInfoStateLRecord )  .  
+ 
+ Declare Instance LocalState_ι_optaddress     : LocalStateField ( XMaybe XAddress )  .  
+ 
+ Declare Instance LocalState_ι_TONTokenWallet     : LocalStateField TONTokenWalletStateLRecord  .  
+ 
+ Declare Instance LocalState_ι_tpladdressGrams     : LocalStateField ( XAddress * XInteger256 (* Grams *) )  .  
+ 
+ Declare Instance LocalState_ι_TvmSlice     : LocalStateField XSlice  .  
+ 
+ Declare Instance LocalState_ι_optOrderRet     : LocalStateField ( XMaybe OrderRetStateLRecord )  .  
+
+Definition LedgerVMStateEmbedded := LedgerStateLEmbeddedType Ledger_ι_VMState . 
+Definition LedgerVMStateField := Ledger_ι_VMState .
+Definition isoVMState := Ledger_ι_VMStateIso.
+
+Definition LedgerMessagesEmbedded := LedgerStateLEmbeddedType Ledger_ι_MessagesAndEvents . 
+Definition LedgerMessagesField := Ledger_ι_MessagesAndEvents .
+Definition isoMessages := Ledger_ι_MessagesAndEventsIso.
+Definition MessagesAndEvents := MessagesAndEventsStateLRecord .
+
+GenerateLocalStateInstances LocalStateStateL LocalStateFieldsI Build_LocalStateField LocalStateStateLEmbeddedType.
+
+Check LocalState_ι_intLocalField.
+Check LocalState_ι_boolLocalField.
+
+Definition LocalStateField_XInteger := LocalState_ι_intLocalField .
+Definition LocalStateField_XBool := LocalState_ι_boolLocalField .
+Definition LocalStateField_XCell := LocalState_ι_cellLocalField .
+
+
+(***************************************)
+Lemma MessagesAndEventsFields_noeq : forall (f1 f2:  MessagesAndEventsFields ) 
+         (v2: field_type f2) (r :  MessagesAndEventsStateLRecord  ) ,  
+f1 <> f2 -> 
+f1 {$$ r with f2 := v2 $$} = f1 r.
+Proof.
+  intros.
+  destruct f1; destruct f2; 
+  (revert r;     
+               apply (countable_prop_proof (T:= MessagesAndEventsStateLRecord ));
+               cbv;
+               first [reflexivity| contradiction]).
+Qed .
+
+Lemma PriceFields_noeq : forall (f1 f2:  PriceFields ) 
+         (v2: field_type f2) (r :  PriceStateLRecord  ) ,  
+f1 <> f2 -> 
+f1 {$$ r with f2 := v2 $$} = f1 r.
+Proof.
+  intros.
+  destruct f1; destruct f2; 
+  (revert r;     
+               apply (countable_prop_proof (T:= PriceStateLRecord ));
+               cbv;
+               first [reflexivity| contradiction]).
+Qed .
+
+Lemma LocalStateFields_noeq : forall (f1 f2:  LocalStateFieldsI ) 
+         (v2: field_type f2) (r :  LocalStateStateLRecord  ) ,  
+f1 <> f2 -> 
+f1 {$$ r with f2 := v2 $$} = f1 r.
+Proof.
+  intros.
+  destruct f1; destruct f2; 
+  (revert r;     
+               apply (countable_prop_proof (T:= LocalStateStateLRecord ));
+               cbv;
+               first [reflexivity| contradiction]).
+Qed .
+
+Lemma LedgerFields_noeq : forall (f1 f2:  LedgerFields ) 
+         (v2: field_type f2) (r :  LedgerStateLRecord  ) ,  
+f1 <> f2 -> 
+f1 {$$ r with f2 := v2 $$} = f1 r.
+Proof.
+  intros.
+  destruct f1; destruct f2; 
+  (revert r;     
+               apply (countable_prop_proof (T:= LedgerStateLRecord ));
+               cbv;
+               first [reflexivity| contradiction]).
+Qed .
+
+End PriceClass .
